Sorting/PairingSort.v
@@ -5,61 +5,73 @@ Require Export PairingHeap.
 
 Set Implicit Arguments.
 
-Fixpoint sum (l : list nat) : nat :=
-match l with
-    | [] => 0
-    | n :: ns => n + sum ns
-end.
-
-Fixpoint size {A : Type} (h : PairingHeap A) : nat :=
-match h with
-    | E => 0
-    | T _ l => S (sum (map size l))
-end.
-
-Lemma size_empty :
-  forall A : Type, size (@empty A) = 0.
-Proof. reflexivity. Qed.
-
-Lemma size_singleton :
-  forall (A : Type) (x : A), size (singleton x) = 1.
-Proof. reflexivity. Qed.
-
-Lemma size_merge :
-  forall (A : Type) (p : A -> A -> bool) (h1 h2 : PairingHeap A),
-    size (merge p h1 h2) = size h1 + size h2.
-Proof.
-  induction h1 using Tree_ind_proper.
-    reflexivity.
-    destruct h2; cbn; try destruct (p x a); cbn; lia.
-Qed.
-
-Lemma size_insert :
-  forall (A : Type) (p : A -> A -> bool) (x : A) (h : PairingHeap A),
-    size (insert p x h) = S (size h).
-Proof.
-  intros. apply size_merge.
-Qed.
-
-Lemma size_mergePairs :
-  forall (A : Type) (p : A -> A -> bool) (l : list (Tree A)),
-    size (mergePairs p l) = sum (map size l).
-Proof.
-  intros. functional induction mergePairs p l; cbn.
-    reflexivity.
-    rewrite <- plus_n_O. reflexivity.
-    rewrite !size_merge, IHp0, plus_assoc. reflexivity.
-Qed.
-
-Check insert.
-
-(* Fixpoint fromList {A : Type} (cmp : A -> A -> bool) (l : list A) : PairingHeap A :=
+Fixpoint fromList {A : Type} (cmp : A -> A -> bool) (l : list A) : PairingHeap A :=
 match l with
     | [] => empty
     | h :: t => insert cmp h (fromList cmp t)
 end.
- *)
 
+Function toList
+  {A : Type} (p : A -> A -> bool) (h : PairingHeap A) {measure size h}: list A :=
+match extractMin p h with
+    | None => []
+    | Some (m, h') => m :: toList p h'
+end.
+Proof.
+  destruct h; cbn; intros; subst; inv teq.
+    rewrite size_mergePairs. apply le_n.
+Defined.
+
+Definition pairingSort (A : Type) (p : A -> A -> bool) (l : list A) : list A :=
+  toList p (fromList p l).
+
+(** Properties of [fromList]. *)
+
+Lemma Elem_fromList :
+  forall (A : Type) (cmp : A -> A -> bool) (x : A) (l : list A),
+    Elem x (fromList cmp l) <-> In x l.
+Proof.
+  induction l as [| h t].
+    split; inv 1.
+    simpl. rewrite Elem_insert'', IHt. firstorder.
+Qed.
+
+Lemma isHeap_fromList :
+  forall (A : Type) (p : A -> A -> bool) (l : list A),
+    isHeap p (fromList p l).
+Proof.
+  induction l as [| h t]; cbn.
+    constructor.
+    apply isHeap_insert. assumption.
+Qed.
+
+Lemma countTree_fromList :
+  forall (A : Type) (cmp : A -> A -> bool) (p : A -> bool) (l : list A),
+    countTree p (fromList cmp l) = count p l.
+Proof.
+  induction l as [| h t].
+    cbn. reflexivity.
+    cbn. destruct (fromList cmp t) eqn: Heq.
+      cbn in *. unfold id. destruct (p h); lia.
+      rewrite <- IHt. destruct (cmp h a); cbn; destruct (p h), (p a); unfold id; lia.
+Qed.
+
+(** Properties of [toList]. *)
+
+Lemma countTree_toList :
+  forall (A : Type) (cmp : A -> A -> comparison) (p : A -> bool) (h : PairingHeap A),
+    isHeap cmp h -> countTree p h = count p (toList cmp h).
+Proof.
+  intros until h.
+  functional induction toList cmp h;
+  destruct h; inv e; cbn; destruct (p m); unfold id; intro.
+    rewrite <- IHl, countTree_mergePairs.
+      reflexivity.
+      apply isHeap_mergePairs. inv H.
+    rewrite <- IHl, countTree_mergePairs.
+      reflexivity.
+      apply isHeap_mergePairs. inv H.
+Qed.
 
 Lemma Sorted_toList :
   forall (A : Type) (cmp : A -> A -> comparison) (h : PairingHeap A),
@@ -68,6 +80,40 @@ Proof.
   intros. functional induction toList cmp h.
     constructor.
     rewrite toList_equation in *. destruct h'; cbn in *; constructor.
-      eapply unT_spec; eauto. erewrite Elem_unT_eq; eauto. cbn. assumption.
-      eapply IHl, isHeap_unT; eauto.
+      eapply extractMin_spec; eauto. erewrite Elem_extractMin_eq; eauto. cbn. assumption.
+      eapply IHl, isHeap_extractMin; eauto.
 Qed.
+
+(** Properties of [pairingSort]. *)
+
+Theorem Sorted_pairingSort :
+  forall (A : Type) (cmp : A -> A -> comparison) (l : list A),
+    Sorted cmp (pairingSort cmp l).
+Proof.
+  intros. unfold pairingSort.
+  apply Sorted_toList, isHeap_fromList.
+Qed.
+
+Lemma perm_pairingSort :
+  forall (A : Type) (cmp : A -> A -> comparison) (l : list A),
+    perm (pairingSort cmp l) l.
+Proof.
+  unfold perm, pairingSort. intros.
+  rewrite <- countTree_toList, countTree_fromList.
+    reflexivity.
+    apply isHeap_fromList.
+Qed.
+
+Theorem Permutation_pairingSort :
+  forall (A : Type) (cmp : A -> A -> comparison) (l : list A),
+    Permutation (pairingSort cmp l) l.
+Proof.
+  intros. apply perm_Permutation, perm_pairingSort.
+Qed.
+
+Instance Sort_pairingSort (A : Type) (cmp : A -> A -> comparison) : Sort cmp :=
+{
+    sort := pairingSort cmp;
+    Sorted_sort := Sorted_pairingSort cmp;
+    Permutation_sort := Permutation_pairingSort cmp;
+}.
