Sorting/GeneralizedInsertionSort.v
@@ -60,3 +60,4 @@ Proof.
   rewrite <- countS_toList, <- countS_fromList.
   reflexivity.
 Qed.
+
